examples/webmodel/Secret.SecString.fst
@@ -77,34 +77,9 @@ let classify #l s l' =
 	  let a:a_string ol' = AString #ol' s in
 	  a)
 
-(* Returns the length of the secret string *)
-val length: #l:secLevel -> s:secString l -> Tot (r:nat{r = String.length(content #l s)})
-let length #l s =
-    match l with
-    | PublicVal -> String.length s
-    | SecretVal ol ->
-      (match s with
-       | AString #ol v -> String.length v)
 
-(* Returns the substring of the secret string *)
-val substr : #l:secLevel -> s:secString l -> i:nat -> n:nat{i + n <= length s} -> Tot (ns:(secString l){length ns = n})
-let substr #l s i n =
-    match l with
-    | PublicVal -> substringImpl s i n (* String.make n (String.sub s i n) *)
-    | SecretVal ol ->
-      (match s with
-       | AString #ol v -> AString #ol (substringImpl v i n (* String.make n (String.sub v i n) *)))
-
-(* Concatenates two secret strings of the same secrecy level *)
-val strcat: #l:secLevel -> s:secString l -> t:secString l
-    	    -> Tot (st:secString l{content st = String.strcat (content s) (content t)})
-let strcat #l s t =
-    match l with
-    | PublicVal -> String.strcat s t
-    | SecretVal ol ->
-      let (AString #ol v1) = s in
-      let (AString #ol v2) = t in
-           AString #ol (String.strcat v1 v2)
+val validSingleSecLevel : secLevel -> Tot bool
+let validSingleSecLevel l = match l with | PublicVal -> true | SecretVal [o] -> true | _ -> false
 
 (* Checks if two secret strings of the same secrecy level are equal *)
 val equal: #l:secLevel -> s:secString l -> t:secString l -> Tot (bool)
@@ -116,15 +91,45 @@ let equal #l s t =
       let (AString #ol v2) = t in
       v1 = v2
       
+(* Returns the length of the secret string *)
+val length: #l:secLevel -> s:secString l -> Tot (r:nat{r = String.length(content #l s)})
+let length #l s = 
+    match l with
+    | PublicVal -> String.length s
+    | SecretVal ol -> 
+      (match s with 
+       | AString #ol v -> String.length v)
+
+(* Returns the substring of the secret string *)
+val substr : #l:secLevel -> s:secString l -> i:nat -> n:nat{i + n <= length s} -> Tot (ns:(secString l){length ns = n})
+let substr #l s i n =
+    match l with
+    | PublicVal -> substringImpl s i n (* String.make n (String.sub s i n) *)
+    | SecretVal ol -> 
+      (match s with 
+       | AString #ol v -> AString #ol (substringImpl v i n (* String.make n (String.sub v i n) *)))
+
+(* Concatenates two secret strings of the same secrecy level *)
+val strcat: #l:secLevel -> s:secString l -> t:secString l
+    	    -> Tot (st:secString l{content st = String.strcat (content s) (content t)})
+let strcat #l s t = 		
+    match l with
+    | PublicVal -> String.strcat s t
+    | SecretVal ol -> 
+      let (AString #ol v1) = s in
+      let (AString #ol v2) = t in
+           AString #ol (String.strcat v1 v2)
+      
 (* assume val randomString: (l:secLevel) -> (n:UInt32.t) -> ST (secString l) *)
 (*        	   (requires (fun _ -> true)) *)
 (* 	   (ensures  (fun h0 s h1 -> h0 == h1 /\ length #l s = UInt32.v n)) *)
 
 (* s1 contains a sublist of s2 *)
 val equalSubLevels : s1:secLevel -> s2:secLevel -> GTot (b:bool)
-let equalSubLevels s1 s2 =
-  (match s1,s2 with
+let equalSubLevels s1 s2 = 
+  (match s1,s2 with 
   | PublicVal, PublicVal -> true
+  | SecretVal sec, PublicVal -> true (* public is less secret than sec *)
   | SecretVal sec, SecretVal sec' -> isSublist sec sec'
   | _, _ -> false
   )
@@ -171,45 +176,45 @@ let rec getSecretOrigin #l s ls =
   | ((|hl,hs|),lo)::tl -> if (hl = l && hs = s) then lo else getSecretOrigin s tl
 
 (* Reclassify the string to an unrelated secrecy level *)
-val canReclassify : #l:secLevel -> secString l -> l':secLevel -> secretOriginList -> Tot bool
-let canReclassify #l s l' ls =
+val canReclassify : #l:secLevel -> secString l -> l':secLevel -> Tot bool
+let canReclassify #l s l' =
   (l = PublicVal) || (* If l is public already, it can be classified to any level *)
-  (let lo = getSecretOrigin #l s ls in
+  (let lo = getSecretOrigin #l s secList in 
   match l' with
   | PublicVal -> false
   | SecretVal ol' -> (List.for_all (fun x -> List.mem x lo) ol'))
 
 val addSecretOrigins : #l:secLevel -> s:secString l -> ol:list torigin -> ls:secretOriginList -> Tot (nls:secretOriginList)
-let rec addSecretOrigins #l s ol ls =
+let rec addSecretOrigins #l s ol ls = 
   match ls with
   | [] -> [((|l, s|), ol)]
   | ((|hl,hs|),lo)::tl -> if (hl = l && hs = s) then ((|hl,hs|), (List.append ol lo))::tl else ((|hl,hs|),lo)::(addSecretOrigins s ol tl)
 
-val reclassify : #l:secLevel -> s:secString l -> l':(secLevel) -> ls:secretOriginList{canReclassify #l s l' ls} -> Tot (t:(secString l'){content t = content s})
-let reclassify #l s l' ls =
+val reclassify : #l:secLevel -> s:secString l -> l':(secLevel){canReclassify #l s l'} -> Tot (t:(secString l'){content t = content s})
+let reclassify #l s l' =
     match l,l' with
     | PublicVal, PublicVal -> s
-    | PublicVal, SecretVal ol -> classify s l'
+    | PublicVal, SecretVal ol -> classify s l'	
     | SecretVal ol, PublicVal -> (match s with | AString #ol t -> t)
-    | SecretVal ol, SecretVal ol' ->
+    | SecretVal ol, SecretVal ol' -> 
 	(match s with | AString #ol s -> let a:a_string ol' = AString #ol' s in a)
 
-(* Declassify a secret string *)
-let declassify (#l:secLevel) (s:secString l) : Tot string =
+(* Checks if the origin is a part of the secrecy level or if the secrecy level is public *)
+let declassify (#l:secLevel) (s:secString l) : Tot string = 
     match l with
     | PublicVal -> s
-    | SecretVal ol ->
+    | SecretVal ol -> 
       let (AString #ol v) = s in v
 
-let rec declassify_list  (#l:secLevel) (s:list (secString l)) : Tot (list string) =
-  match s with
+let rec declassify_list  (#l:secLevel) (s:list (secString l)) : Tot (list string) = 
+  match s with 
   | [] -> []
   | hd::tl -> (declassify #l hd)::(declassify_list tl)
 
 (* for printing and logging *)
 val getOriginString : list torigin -> Tot (string)
 let rec getOriginString l =
-  match l with
+  match l with 
   | [] -> ""
   | hd::tl -> "Origin: " ^ (origin_to_string hd) ^ "\n" ^ (getOriginString tl)
   
