examples/webmodel/NetworkRequestInterface.fst
@@ -1,0 +1,194 @@
+module NetworkRequestInterface
+
+open FStar.IO
+open Web.Origin
+open Web.URI
+open Secret.SecString
+open Browser.AuxiliaryDatatypes
+open Browser.Datatypes
+open AuxiliaryFunctions
+open Browser.StringFunctions
+open Browser.Model.Interface
+open ML.ExternalFunctions
+
+module List = FStar.List.Tot
+
+(* the secrets are indexed by a list of origins --- state, authcode, accesstoken, client_secret, password *)
+type secretVal =
+| Secret : s:secLevel -> v:secString s -> secretVal
+
+(* default responses *)
+let defResponse = ActResponse PublicVal ({resptype="default";respcode=200;respurl=[];resphead=[];respbody=(emptyString PublicVal);resptrail=[];respHTTPS="none";respCSP=[];respCORS=[];resploc=None;respRedSec=PublicVal})
+let defErrResponse = ActResponse PublicVal ({resptype="default";respcode=404;respurl=[];resphead=[];respbody=(emptyString PublicVal);resptrail=[];respHTTPS="none";respCSP=[];respCORS=[];resploc=None;respRedSec=PublicVal})
+
+val mk_secretval : #l:secLevel -> secString l -> Tot secretVal
+let mk_secretval #l s = (Secret l s)
+
+val mk_svheaderval : secretVal -> Tot headervalue
+let mk_svheaderval s = Headervalue (Secret?.s s) (Secret?.v s)
+
+val genSecret : l:secLevel -> Tot (s:secretVal{Secret?.s s = l})
+let genSecret l = Secret l (classify #PublicVal (randomVal 32) l) (* Generate random-string of length 32 *)
+
+val getSecret : #l:secLevel -> s:secretVal{Secret?.s s = l} -> Tot (secString l)
+let getSecret #l s = (Secret?.v s)
+
+(* Server-side checks for equality of two strings *)
+val s_equal: #l:secLevel -> #l':secLevel -> s:secString l -> t:secString l' -> Tot (b:bool{b = true ==> content s = content t})
+let s_equal #l #l' s t = 
+  match l, l' with
+  | PublicVal, PublicVal -> s = t
+  | SecretVal ol, PublicVal -> let (AString #ol v1) = s in v1 = t
+  | PublicVal, SecretVal ol -> let (AString #ol v2) = t in s = v2
+  | SecretVal ol, SecretVal ol' ->
+      let (AString #ol v1) = s in
+      let (AString #ol' v2) = t in
+      v1 = v2
+
+val compareSecret : s:secretVal -> t:secretVal -> Tot (b:bool)
+let compareSecret s t = s_equal (Secret?.v s) (Secret?.v t)
+
+(* TRUSTED ORIGINS *)
+val trustedOrigins : list torigin
+
+let ipori = TOrigin "https" ["login";"ip";"com"] (Some 443) None
+let rpori = TOrigin "https" ["rp";"com"] (Some 443) None
+let badipori = TOrigin "https" ["login";"badip";"com"] (Some 443) None
+
+let trustedOrigins = [ipori;rpori]
+
+(* Is the uri from a list of origins specified *)
+private val isTrusted : list torigin -> uri -> Tot bool
+let rec isTrusted t u = 
+  match t with
+  | [] -> false
+  | h::tl -> (isSameOriginUO u h) || (isTrusted tl u)
+
+(* Is the window from a trustedOrigin? *)
+val isTrustedOriginWindow : cowindow -> Tot bool
+let isTrustedOriginWindow cw =
+  let wurl = getWinURI cw in
+  isTrusted trustedOrigins wurl 
+
+
+(* retrieve the value from the querystring (also cookie name value) that corresponds to the given string str *)
+val getVal : #l:secLevel -> list (secString l * secString l) -> secString l -> Tot (secString l)
+let rec getVal #l qs str = 
+  match qs with
+  | [] -> emptyString l
+  | (f,s)::tl -> if (f=str) then (s) else getVal tl str
+
+(* retrieve the value from the querystring (also cookie name value) that corresponds to the given string str *)
+val getQSVal : #l:secLevel -> querystring l -> string -> Tot (secString l)
+let getQSVal #l qs str = getVal #l qs (classify #PublicVal str l)
+
+
+(* Leak values which the adversary can access - declassify the value to the attacker *)
+val leakValue : headervalue -> Tot string
+let leakValue hv = 
+  match (Headervalue?.hvs hv) with 
+  | PublicVal -> s_getHeaderValueString #PublicVal hv
+  | SecretVal lo -> 
+      if (List.for_all (fun x -> List.mem x trustedOrigins) lo) then "" 
+      else declassify (s_getHeaderValueString #(SecretVal lo) hv)
+
+(* Coerce values to an attacker defined index *)
+val coerceValue : string -> l:(list torigin){not (emptyList l)} -> Tot headervalue
+let coerceValue s l = Headervalue (SecretVal l) (classify #PublicVal s (SecretVal l))
+
+private val getWinList : list cowindow -> Tot (list cowindow)
+let rec getWinList l = 
+  match l with
+  | [] -> []
+  | hd::tl -> List.append (getWinList (getFrames hd)) (getWinList tl)
+
+private val getWindows : browser -> Tot (list cowindow)
+let getWindows b = getWinList b.windows
+
+val checkEP : request -> string -> Tot bool
+let checkEP r s = 
+  let ruri = (firstElement (Request?.rf r).requrl) in
+  match getPathVal #(URI?.usl ruri) (ruri) with
+  | [] -> false
+  | h::_ -> eqString h s
+  
+
+
+
+(* ***** Browser Exposed Functions ***** *)
+val getAllWindows : b:browser -> Tot (list cowindow)
+let getAllWindows b = getWindows b
+
+type execWindow = sw:window{List.find (fun w -> w = SB_Script) sw.wsbox = None}
+
+val getWin : cowindow -> Tot (option execWindow)
+let getWin cw =
+  if (isTrustedOriginWindow cw) then None
+  else if (List.find (fun w -> w = SB_Script) (CWindow?.cwsbox cw) <> None) then None
+  else Some (cowin_to_win cw) (* Need to expose the function here *)
+
+val getDocumentDomain : browser -> execWindow -> Tot (hdomain)
+let getDocumentDomain b sw = (get_document_domain b sw)
+
+val setDocumentDomain : browser -> execWindow -> hdomain -> Tot (browser * cowindow)
+let setDocumentDomain b sw hd =
+    let (r, w, nb) = (set_document_domain b sw hd) in
+    (nb, win_to_cowin w)
+
+val getWinLocation : #s:secLevel -> browser -> execWindow -> cowindow -> Tot (option (c_uri s))
+let getWinLocation #s b sw cw =
+  let (r, u) = get_win_location b (win_to_cowin sw) cw in
+  u
+
+val setWinLocation : browser -> execWindow -> cowindow -> u:uri{match (URI?.usl u) with | SecretVal [o] -> true | _ -> false} -> Tot browser
+let setWinLocation b sw cw u =
+  let (r, req, w, nb) = set_win_location b (win_to_cowin sw) cw u in
+  nb
+
+val getLocalStorageItem : browser -> execWindow -> string -> Tot string
+let getLocalStorageItem b sw key =
+  let (r, v) = (get_item_localStorage b sw None key) in
+  v
+
+val setLocalStorageItem : browser -> execWindow -> string -> string -> Tot browser
+let setLocalStorageItem b sw key value =
+  let (r, nb) = (set_item_localStorage b sw None key value) in
+  nb
+
+val postMessage : browser -> execWindow -> cowindow -> string -> string -> Tot result
+let postMessage b sw cw msg ori = post_message b (win_to_cowin sw) cw msg ori
+
+val getWinByName : browser -> execWindow -> string -> Tot (browser * cowindow)
+let getWinByName b sw n =
+  let (r, cw, nb) = get_window_from_name b (win_to_cowin sw) n in
+  (nb, cw)
+
+val winOpen : browser -> execWindow -> string -> string -> Tot (browser * cowindow)
+let winOpen b sw u n =
+  let (r, req, cw, nb) = open_window b (win_to_cowin sw) u n in
+  (nb, cw)
+
+val winClose : browser -> execWindow -> cowindow -> Tot browser
+let winClose b sw cw = close_window b (sw) cw
+  
+
+(* val processNextResponse : browser -> cowindow -> actResponse -> bool -> result *)
+(* let processNextResponse b cw resp f = *)
+(*   if (not (isTrustedOriginWindow cw) && Some? (getWin cw)) then  *)
+(*     let win = (Some?.v (getWin cw)) in *)
+(*     let conn = (mk_connection ({cori=win.wloc.c_origin;ccred=f})) in *)
+(*     let (r, nb) = processResponse b conn resp in *)
+(*     b := nb; r *)
+(*   else  *)
+(*     ( *)
+(*     let win = cowin_to_win cw in  *)
+(*     let conn = (mk_connection ({cori=win.wloc.c_origin;ccred=f})) in *)
+(*     let respconn = getResponseConn (b).conn conn in *)
+(*     match respconn with *)
+(*     | None -> Success "" *)
+(*     | Some ((req,sw,tw,ty), f, ncl) ->  *)
+(* 	let f = getProcResponse win.wloc.c_origin in  *)
+(* 	let (r, nb) = processResponse b conn (f req) in *)
+(* 	Success "" *)
+(*     )  *)   
+
