examples/webmodel/OAuth.IP.fst
@@ -1,0 +1,140 @@
+module OAuth.IP
+
+open FStar.All
+open FStar.Heap
+open FStar.IO
+open Web.Origin
+open Web.URI
+open Secret.SecString
+open Browser.AuxiliaryDatatypes
+open Browser.Datatypes
+open AuxiliaryFunctions
+open Browser.StringFunctions
+open Browser.Model.Interface
+open NetworkRequestInterface
+open OAuth.Datatypes
+
+(* ***** IP.COM ***** *)
+let ipurl = ({c_origin=ipori;c_uname=emptyString (SecretVal [ipori]);c_pwd=emptyString (SecretVal [ipori]);c_path=[];c_querystring=[];c_fragment=emptyString (SecretVal [ipori])})
+let ipuri = mk_uri ipurl
+
+val checkIPReq : req:request -> Tot (b:bool)
+let checkIPReq req =
+  match (Request?.rsl req) with
+  | PublicVal -> true
+  | SecretVal ol -> List.mem ipori ol
+
+val ipReqLemma : req:request -> Lemma (requires (checkIPReq req)) (ensures (restricts (Request?.rsl req) (SecretVal [ipori]))) [SMTPat (checkIPReq req)]
+let ipReqLemma req = ()
+
+(* check the validity of the session id *)
+val isValid : #l:secLevel -> list (secString l) -> string -> Tot bool
+let rec isValid #l ls s = 
+  match ls with
+    | [] -> false
+    | hd::tl -> eqString (hd) s || isValid tl s
+  
+val isValidSessionId : #l:secLevel -> uList l -> string -> Tot bool
+let rec isValidSessionId #l sl s = 
+  match sl with
+    | [] -> false
+    | (_,_,c)::tl -> isValid c s || isValidSessionId tl s 
+
+(* check the validity of the password *)
+val isValidPwd : #l:secLevel -> #l':secLevel -> uList (SecretVal [ipori]) -> (secString l) -> (secString l') -> Tot bool
+let rec isValidPwd #l #l' sl su sp = 
+  match sl with
+    | [] -> false
+    | (u,p,_)::tl -> if (s_equal u su) then (s_equal p sp) else isValidPwd tl su sp 
+    
+val isAlreadyLoggedIn : uList (SecretVal [ipori]) -> list (string * string) -> Tot bool
+let isAlreadyLoggedIn ul l = isValidSessionId ul (getVal #PublicVal l "_ipsid")
+
+val authenticateUser : uList (SecretVal [ipori]) -> req:request -> Tot bool
+let authenticateUser ul req =
+  let s = (s_getRequestBody #(Request?.rsl req) req) in
+  let qs = getFormData s in
+  isValidPwd ul (getQSVal qs "user") (getQSVal qs "pwd")
+		    
+(* authentication of the user - return the authcode along with the state to the RP *)
+val getIPAuthResp : r:request -> ML (resp:actResponse{requestResponseValid r resp})
+let getIPAuthResp r =
+    let rsl = s_getReqURISecLevel r in
+    let ruri = s_getRequestURI r in
+    let ul = !userList in 
+    if ((isAlreadyLoggedIn ul (getReqCookie (s_getReqHeaderValue r "Cookie"))) ||
+       ((Request?.rf r).reqm = "POST" && (authenticateUser ul r))) then
+       let cid = declassify (getQSVal ruri.c_querystring "client_id") in
+       let reduri = s_secstring_uri #PublicVal (declassify (getQSVal ruri.c_querystring "redirect_uri")) in 
+       match reduri with 
+       | None -> (print_string ("Error:getIPAuthResp - getRPOrigin \n");defErrResponse)
+       | Some (o,red) -> (* && (getRPOrigin cid = (s_getURI (Some?.v reduri)).c_origin) ) then ( check for origins to be the same? *)
+	 let urisl = SecretVal [o] in
+	 let rori = declassify (getQSVal #rsl ruri.c_querystring "origin") in
+	 let token = classify #PublicVal (declassify (getQSVal #rsl ruri.c_querystring "csrftoken")) urisl in
+	 let authcode = genSecret urisl in
+	 let ipREP = curi_to_hstring ({c_origin=red.c_origin;c_uname=classify red.c_uname urisl;c_pwd=classify red.c_pwd urisl;c_path=classifyPath red.c_path urisl;c_querystring=[(classify #PublicVal "authcode" urisl, getSecret (authcode));(classify #PublicVal "csrftoken" urisl, token);(classify #PublicVal "IP" urisl,classify #PublicVal (origin_to_string ipori) urisl)];c_fragment=emptyString urisl}) in
+	 let stateToken = Secret urisl token in 
+	 let rduri = mk_uri red in
+	 ipCL := (o, stateToken, authcode, rduri)::(!ipCL);
+	 (
+	 (* ******* For redirect-attack, change the respcode here to 307 or 308 ******* *)
+	 let ck = genSecret (SecretVal [ipori]) in
+	 let chead = (if (emptyList (getReqCookie (s_getReqHeaderValue r "Cookie"))) then [("Set-Cookie", (mk_svheaderval ck))] else []) in
+	 let nhead = ("Location", (mk_headerval #urisl ipREP))::chead in
+	 ActResponse (SecretVal [o;ipori]) ({resptype="default";respcode=303;respurl=[];resphead=nhead;respbody=(emptyString (SecretVal [o;ipori]));resptrail=[];respHTTPS="modern";respCSP=cspPol;respCORS=[];resploc=None;respRedSec=urisl})
+	 )	 
+    else if ((Request?.rf r).reqm = "GET") then (* send login form for authentication *)
+    (
+       let cid = declassify (getQSVal ruri.c_querystring "client_id") in
+       if (getRPOrigin cid = s_getRequestOrigin r) then 
+	 ActResponse (SecretVal [ipori]) ({resptype="default";respcode=200;respurl=[];resphead=[];respbody=(emptyString (SecretVal [ipori]));resptrail=[];respHTTPS="modern";respCSP=cspPol;respCORS=[];resploc=None;respRedSec=PublicVal})
+       else
+	 defErrResponse
+    )
+    else
+	(print_string ("Error:getIPAuthResp \n"); defErrResponse) (* Authenticate user - send a redirect response to authentication page *)
+	
+(* check the authcode from the RP and then send the access_token *)
+val getIPTokenResp : r:request -> ML (resp:actResponse{requestResponseValid r resp})
+let getIPTokenResp r =
+    let urisl = s_getReqURISecLevel r in
+    let ruri = s_getRequestURI r in
+    let cid = declassify (getQSVal ruri.c_querystring "client_id") in
+    let reduri = secstring_to_uri #urisl (getQSVal ruri.c_querystring "redirect_uri") in
+    let rorig = getRPOrigin cid in
+    let olist = (SecretVal [ipori;rorig]) in
+    let cs = (getQSVal ruri.c_querystring "client_secret") in
+    let code = (getQSVal ruri.c_querystring "authcode") in
+    let clcode = (getCLCode !ipCL rorig) in
+    let cdsec = (getCDSecret !ipCD rorig) in
+    let red_uri = (getCLRedURI !ipCL rorig) in
+    match clcode, cdsec with
+    | None, _ -> defErrResponse
+    | _, None -> defErrResponse
+    | Some ccode, Some csec -> (
+	   if ((rorig = s_getRequestOrigin r) && (compareSecret (mk_secretval code) ccode) && (compareSecret (mk_secretval cs) csec) &&
+	      (Some? reduri) && (Some? red_uri) && (Some?.v red_uri = Some?.v reduri)) then (
+	      let tokenS = genSecret olist in
+	      ipCL := (getNewCodeList !ipCL rorig ccode (Some?.v red_uri));
+	      ipTL := (rorig, tokenS)::(!ipTL);
+	      let atoken = getSecret tokenS in 
+	      let rbody = strcat (classify #PublicVal "access_token:" olist) atoken in
+	      let ipResp = ActResponse olist ({resptype="default";respcode=200;respurl=[];resphead=[];respbody=rbody;resptrail=[];respHTTPS="modern";respCSP=cspPol;respCORS=[];resploc=None;respRedSec=PublicVal}) in
+	      ipResp)
+	   else
+	      defErrResponse)
+
+val ipReqResp : req:request -> ML (ret:retReqResp{isValidRetResp req ret})
+let ipReqResp r =
+    let urisl = s_getReqURISecLevel r in
+    let ruri = s_getRequestURI #urisl r in (* get the request url *)
+    if checkIPReq r && (getPort (mk_uri ruri)) = (Some 443) then (* Only accept secure connections (HTTPS) *)
+    (
+      if (checkEP r "authEP") then (* check for cookies and then either get user-data or send redirection url *)
+	(RetResponse (getIPAuthResp r))
+      else if (checkEP r "tokenEP") then (RetResponse (getIPTokenResp r))
+      else (RetResponse defErrResponse)
+      )
+    else
+      (RetResponse defErrResponse)
