examples/webmodel/OAuth.User.fst
@@ -1,0 +1,183 @@
+module OAuth.User
+
+open FStar.All
+open FStar.Heap
+open FStar.IO
+open Web.Origin
+open Web.URI
+open Secret.SecString
+open Browser.AuxiliaryDatatypes
+open Browser.Datatypes
+open AuxiliaryFunctions
+open Browser.StringFunctions
+open Browser.Model.Interface
+open NetworkRequestInterface
+open OAuth.Datatypes
+open OAuth.RP
+open OAuth.IP
+
+val anyReqResp : r:request -> Tot (ret:retReqResp{isValidRetResp r ret})
+let anyReqResp r = RetResponse defResponse
+
+val getResponse : o:torigin{List.mem o trustedOrigins} -> ML (r:request -> ML (ret:retReqResp{isValidRetResp r ret}))
+let getResponse o =
+  if (o = rpori) then rpReqResp
+  else if (o = ipori) then ipReqResp
+  else anyReqResp
+
+val getProcResponse : o:origin -> ML (r:request -> ML (ret:retReqResp{isValidRetResp r ret}))
+let getProcResponse o = 
+  if (TOrigin? o && List.mem o trustedOrigins) then getResponse o
+  else anyReqResp
+
+let b = (init_browser)
+let (i, nb) = (set_unique_id b)
+
+(* Window's origin - RP to log into *)
+let ori = TOrigin "https" ["rp";"com"] (Some 443) None
+let durl = {c_origin=ori;c_uname=emptyString (SecretVal [ori]);c_pwd=emptyString (SecretVal [ori]);c_path=[];c_querystring=[];c_fragment=emptyString (SecretVal [ori])}
+let duri = mk_uri durl
+let doc = {dloc=duri;dref=blank_uri;dori=(mk_aorigin durl.c_origin);dHTTPS="none";drefPol=RP_NoReferrer;dCSP=[];dsbox=[];}
+let (sw, cb) = 
+      let hist = HistEntry (URI?.usl duri) (URI?.u duri) get_time doc i in 
+      let newwin = (win_to_cowin ({winid=i;wname="";wloc=duri;wframes=[];wopener=None;wparent=None;whist={hlhe=[hist];hcur=1};wdoc=(doc);wsbox=[];})) in
+      (newwin, ({(nb) with windows=newwin::(nb).windows}))
+
+let sl = (SecretVal [rpori])
+(* Request's URL - RP's server *)
+let rurl = {c_origin=rpori;c_uname=emptyString sl;c_pwd=emptyString sl;c_path=[(classify #PublicVal "login-ipauth" sl)];c_querystring=[(classify #PublicVal "IP" sl),(classify #PublicVal "ip.com" sl)];c_fragment=emptyString sl}
+let ruri = mk_uri rurl
+(* Request to start OAuth authentication *)
+let newreq = Request sl ({reqm = "POST"; requrl = [ruri]; reqhead = []; reqo = (mk_aorigin (URI?.u (CWindow?.cwloc sw)).c_origin); reqw = (Some sw); reqinit = ""; reqtype = ""; reqdest = ""; reqtarget = None; reqredirect = 0; reqredmode = "follow"; reqref = (Client sw); reqrefPolicy = RP_OriginWhenCO; reqnonce = ""; reqparser = ""; requnsafe = false; reqpreflight = false; reqsync = false; reqmode = NoCORS; reqtaint = "basic"; reqcredm = "omit"; reqcredflag = false; reqbody = emptyString sl; corsflag = false; corspfflag = false; authflag = false; recflag = false})
+
+(* Username and password for IP *)
+let uname = classify #PublicVal "usernameU" (SecretVal [ipori])
+let pass = classify #PublicVal "passwordP" (SecretVal [ipori])
+
+val print_result : result -> ML unit
+let print_result r =
+  match r with 
+  | Error e -> print_string ("Error: " ^ e ^ "\n")
+  | Success s -> print_string ("Success: " ^ s ^ "\n")
+
+val processRPResponse : req:request{notForbiddenHeaderfieldInReqHeader (Request?.rf req).reqhead} -> ML (result * browser) 
+let processRPResponse req = 
+  let pr' = (getProcResponse rpori) req in
+  match pr' with
+  | RetRequest nreq -> (let co = {cori=ipori;ccred=true} in
+		      match (getConnection !rpb co) with (* the rp creates a new request here - sent to the ip *)
+		      | None -> (Error ("No connections available!"), !rpb)
+	   	      | Some ({connect=oconn;creq=oreq}) -> 
+			     let pr'' = (getProcResponse ipori) nreq in
+			     (match pr'' with 
+			     | RetRequest _ -> (Error ("No response from ipori!"), !rpb) 
+			     | RetResponse pr -> let (res, _, _, nb) = processResponse !rpb oconn nreq pr in 
+						(res,nb)))
+  | RetResponse _ -> (Error ("No request made from RP to IP!"), !rpb) 
+
+(* Process the response from the IP after authentication *)
+val processIPResponse : browser -> req:request{notForbiddenHeaderfieldInReqHeader (Request?.rf req).reqhead} -> ML (result * browser) 
+let processIPResponse ib req =
+    let co = {cori=ipori;ccred=true} in
+    match (getConnection ib co) with
+    | None -> (Error ("No connections available!"), ib)
+    | Some ({connect=oconn;creq=oreq}) ->
+	let pr' = (getProcResponse ipori) req in
+	match pr' with
+	| RetRequest _ -> (Error ("No connections available!"), ib)
+	| RetResponse pr ->
+	    let (res, nr, _, nb) = processResponse ib oconn req pr in 
+	    (
+	    print_result res; 
+	    match nr with
+	    | None -> (Success ("No more requests!"), nb)
+	    | Some nreq -> processRPResponse nreq)
+			  (* (let pr = (getProcResponse rpori) nreq in *)
+			  (* match (getConnection !rpb co) with (\* the rp creates a new request here - sent to the ip *\) *)
+			  (* | None -> (Error ("No connections available!"), !rpb) *)
+			  (* | Some ({connect=oconn;creq=oreq}) -> ( *)
+			  (* 	 match (oreq) with  *)
+			  (* 	 | [] -> (Error ("No requests on connection for IP!"), !rpb) *)
+			  (* 	 | (rq,_,_,_)::_ -> ((\* remove the headers that should not be a part of request (redirect) *\) *)
+			  (* 	     let nrq = (Request (Request?.rsl rq) ({(Request?.rf rq) with reqhead=(redirectHeaders (Request?.rf rq).reqhead)})) in *)
+			  (* 	     let pr = (getProcResponse ipori) nrq in *)
+			  (* 	     let (res, _, _, nb) = processResponse !rpb oconn nrq pr in  *)
+			  (* 	     (res, !rpb))))) *)
+
+let ipsl = SecretVal [ipori]
+let formurl = {c_origin=ipori;c_uname=emptyString ipsl;c_pwd=emptyString ipsl;c_path=[(classify #PublicVal "authEP" ipsl)];c_querystring=[];c_fragment=emptyString ipsl}
+let formuri = mk_uri formurl
+
+val processIPFormResponse : browser -> req:request{notForbiddenHeaderfieldInReqHeader (Request?.rf req).reqhead} -> connection -> ML (result * browser)
+let processIPFormResponse br r oconn =
+  let pr'' = (getProcResponse ipori) r in
+  match pr'' with 
+  | RetRequest _ -> (Error ("Request should not occur."), br)
+  | RetResponse pr -> let (res, nr', w, nbr) = processResponse br oconn r pr in (* response from ip processed - requires submission of form*)
+	(print_result res;
+	match w with
+	| None ->  (Error ("No executable window!\n"), nbr)
+	| Some sw -> 
+	    (let qsfd = [(classify #PublicVal "user" ipsl, classify #PublicVal "usernameU" ipsl);(classify #PublicVal "pwd" ipsl, classify #PublicVal "passwordP" ipsl)] in
+	    let (_, nr', _, nb) = form_submission nbr (cowin_to_win sw) "" "POST" formuri qsfd in
+	    match nr' with 
+	    | None -> (Error ("No proper request!\n"), nbr)
+	    | Some req -> processIPResponse nb req))
+
+let browserOAuth () : ML (result * browser) =
+  let (r, _, nw, nb) = open_window cb sw "https://rp.com/" "" in
+  let (re, nr, win, sb) = navigateWindow (nb) sw nw (RequestResource newreq) "other" in
+  match sb.conn with (*the response arrives on the connection - assume connection is the first available here*)
+  | [] -> (Error ("No connections"), sb)
+  | hd::_ ->
+      let pr' = (getProcResponse rpori) newreq in
+      match pr' with
+      | RetRequest _ -> (Error ("No proper response!"), sb)
+      | RetResponse pr -> let (r1, nr, _, br) = processResponse sb (getConn hd).connect newreq pr in (* Processes response from RP that redirects to IP *)
+	  (print_result r1;
+	  let co = {cori=ipori; ccred=true} in
+	  match (getConnection br co) with
+	  | None -> (Error ("No connections after response from RP to IP"), br)
+	  | Some ({connect=oconn;creq=oreq}) -> (
+		 match nr with 
+		 | None -> (Error ("No requests made here"), br)
+		 | Some nreq -> processIPFormResponse br nreq oconn))
+
+(* Request's URL - RP's server - Assuming that the initial request was for "ip.com" but attacker modified it to "badip.com" *)
+(* Everything else happens at ip.com *)
+let birurl = {c_origin=rpori;c_uname=emptyString sl;c_pwd=emptyString sl;c_path=[(classify #PublicVal "login-ipauth" sl)];c_querystring=[(classify #PublicVal "IP" sl),(classify #PublicVal "badip.com" sl)];c_fragment=emptyString sl}
+let biruri = mk_uri birurl
+(* Request to start OAuth authentication *)
+let bireq = Request sl ({reqm = "POST"; requrl = [biruri]; reqhead = []; reqo = (mk_aorigin (URI?.u (CWindow?.cwloc sw)).c_origin); reqw = (Some sw); reqinit = ""; reqtype = ""; reqdest = ""; reqtarget = None; reqredirect = 0; reqredmode = "follow"; reqref = (Client sw); reqrefPolicy = RP_OriginWhenCO; reqnonce = ""; reqparser = ""; requnsafe = false; reqpreflight = false; reqsync = false; reqmode = NoCORS; reqtaint = "basic"; reqcredm = "omit"; reqcredflag = false; reqbody = emptyString sl; corsflag = false; corspfflag = false; authflag = false; recflag = false})
+
+(* let ipMixUp () : ML (result * browser) =  *)
+(*   let (r, nw, nb) = open_window cb sw "https://rp.com/" "" in *)
+(*   let (re, win, sb) = navigateWindow (nb) sw nw (RequestResource bireq) "other" in  *)
+(*   match sb.conn with (\*the response arrives on the connection - assume connection is the first available here*\) *)
+(*   | [] -> (Error ("No connections"), sb) *)
+(*   | hd::_ -> *)
+(*       let pr = (getProcResponse rpori) bireq in *)
+(*       let (r1, _, br) = processResponse sb (getConn hd).connect pr in (\* Processes response from RP that redirects to IP *\) *)
+(*       ( *)
+(*       print_result r1; *)
+(*       let co = {cori=ipori; ccred=true} in *)
+(*       match (getConnection br co) with *)
+(*       | None -> (Error ("No connections after response from RP to IP"), br) *)
+(*       | Some ({connect=oconn;creq=oreq}) -> ( *)
+(* 	  match (oreq) with  *)
+(* 	  | [] -> (Error ("No requests on the connection after response from RP to IP"), br) *)
+(* 	  | (rq,_,_,_)::_ -> *)
+(* 	      let pr = (getProcResponse ipori) rq in *)
+(* 	      let (res, w, nbr) = processResponse br oconn pr in (\* response from ip processed - requires submission of form*\)  *)
+(* 	      ( *)
+(* 	      print_result res; *)
+(* 	      match w with  *)
+(* 	      | None ->  (Error ("No executable window!\n"), nbr)  *)
+(* 	      | Some sw -> let (_, _, nb) = form_submission nbr (cowin_to_win sw) "" "POST" None [("user","usernameU");("pwd","passwordP")] in *)
+(* 			  processIPResponse nb *)
+(* 			  ))) *)
+			  
+let main =
+    let (r,nb) = browserOAuth () in
+    print_result r
+	    
